Add sums to compilation and backtranslation

rupicola/stlc/Backtranslation.fst
@@ -10,120 +10,152 @@ open ExpRel
 
 noeq
 type typing : typ_env -> exp -> qType -> Type =
-  | TyUnit : #g:typ_env ->
-             typing g EUnit qUnit
-  | TyTrue : #g:typ_env ->
-             typing g ETrue qBool
-  | TyFalse : #g:typ_env ->
-              typing g EFalse qBool
-  | TyIf : #g:typ_env ->
-           #e1:exp ->
-           #e2:exp ->
-           #e3:exp ->
-           #t:qType ->
-           $h1:typing g e1 qBool ->
-           $h2:typing g e2 t ->
-           $h3:typing g e3 t ->
-             typing g (EIf e1 e2 e3) t
-  | TyVar : #g:typ_env ->
-            x:var{Some? (g x)} ->
-              typing g (EVar x) (Some?.v (g x))
-  | TyLam : #g:typ_env ->
-            #body:exp ->
-            #t1:qType ->
-            #t2:qType ->
-            $hbody:typing (extend t1 g) body t2 ->
-              typing g (ELam body) (t1 ^-> t2)
-  | TyApp : #g:typ_env ->
-            #e1:exp ->
-            #e2:exp ->
-            #t1:qType ->
-            #t2:qType ->
-            $h1:typing g e1 (t1 ^-> t2) ->
-            $h2:typing g e2 t1 ->
-              typing g (EApp e1 e2) t2
-  | TyPair : #g:typ_env ->
-            #e1:exp ->
-            #e2:exp ->
-            #t1:qType ->
-            #t2:qType ->
-            $h1:typing g e1 t1 ->
-            $h2:typing g e2 t2 ->
-              typing g (EPair e1 e2) (t1 ^* t2)
-  | TyFst : #g:typ_env ->
-            #e:exp ->
-            #t1:qType ->
-            #t2:qType ->
-            $h1:typing g e (t1 ^* t2) ->
-              typing g (EFst e) t1
-  | TySnd : #g:typ_env ->
-            #e:exp ->
-            #t1:qType ->
-            #t2:qType ->
-            $h1:typing g e (t1 ^* t2) ->
-              typing g (ESnd e) t2
+| TyUnit : #g:typ_env ->
+           typing g EUnit qUnit
+| TyTrue : #g:typ_env ->
+           typing g ETrue qBool
+| TyFalse : #g:typ_env ->
+            typing g EFalse qBool
+| TyIf : #g:typ_env ->
+         #e1:exp ->
+         #e2:exp ->
+         #e3:exp ->
+         #t:qType ->
+         $h1:typing g e1 qBool ->
+         $h2:typing g e2 t ->
+         $h3:typing g e3 t ->
+         typing g (EIf e1 e2 e3) t
+| TyVar : #g:typ_env ->
+          x:var{Some? (g x)} ->
+          typing g (EVar x) (Some?.v (g x))
+| TyLam : #t1:qType ->
+          #t2:qType ->
+          #body:exp ->
+          #g:typ_env ->
+          $hbody:typing (extend t1 g) body t2 ->
+          typing g (ELam body) (t1 ^-> t2)
+| TyApp : #t1:qType ->
+          #t2:qType ->
+          #e1:exp ->
+          #e2:exp ->
+          #g:typ_env ->
+          $h1:typing g e1 (t1 ^-> t2) ->
+          $h2:typing g e2 t1 ->
+          typing g (EApp e1 e2) t2
+| TyPair : #g:typ_env ->
+          #e1:exp ->
+          #e2:exp ->
+          #t1:qType ->
+          #t2:qType ->
+          $h1:typing g e1 t1 ->
+          $h2:typing g e2 t2 ->
+          typing g (EPair e1 e2) (t1 ^* t2)
+| TyFst : #t1:qType ->
+          #t2:qType ->
+          #e:exp ->
+          #g:typ_env ->
+          $h1:typing g e (t1 ^* t2) ->
+          typing g (EFst e) t1
+| TySnd : #t2:qType ->
+          #t1:qType ->
+          #e:exp ->
+          #g:typ_env ->
+          $h1:typing g e (t1 ^* t2) ->
+          typing g (ESnd e) t2
+| TyInl : #t1:qType ->
+          t2:qType ->
+          #e:exp ->
+          #g:typ_env ->
+          $h:typing g e t1 ->
+          typing g (EInl e) (t1 ^+ t2)
+| TyInr :
+          t1:qType ->
+          #t2:qType ->
+          #e:exp ->
+          #g:typ_env ->
+          $h:typing g e t2 ->
+          typing g (EInr e) (t1 ^+ t2)
+| TyCase : #t1:qType ->
+           #t2:qType ->
+           #t3:qType ->
+           #cond:exp ->
+           #inlc:exp ->
+           #inrc:exp ->
+           #g:typ_env ->
+           $h1:typing g cond (t1 ^+ t2) ->
+           $h2:typing (extend t1 g) inlc t3 ->
+           $h3:typing (extend t2 g) inrc t3 ->
+           typing g (ECase cond inlc inrc) t3
 
-let rec backtranslate (g:typ_env) (e:exp) (t:qType) (h:typing g e t) (fs_g:eval_env g) : (get_Type t) =
+let rec backtranslate (#g:typ_env) (#e:exp) (#t:qType) (h:typing g e t) (fs_g:eval_env g) : (get_Type t) =
   match e with
   | EUnit -> ()
   | ETrue -> true
   | EFalse -> false
-  | EIf e1 e2 e3 ->
-    let TyIf #_ #_ #_ #_ #t h1 h2 h3 = h in
-    let b : bool = backtranslate g e1 qBool h1 fs_g in
-    let v1 = backtranslate g e2 t h2 fs_g in
-    let v2 = backtranslate g e3 t h3 fs_g in
-    if b then v1 else v2
+  | EIf _ _ _ ->
+    let TyIf h1 h2 h3 = h in
+    if backtranslate h1 fs_g
+    then backtranslate h2 fs_g
+    else backtranslate h3 fs_g
   | EVar x -> index fs_g x
-  | ELam body ->
-    let TyLam #_ #_ #t1 #t2 hbody = h in
+  | ELam _ ->
+    let TyLam #t1 #t2 hbody = h in
     assert (t == (t1 ^-> t2));
     let w : (get_Type t1) -> (get_Type t2) =
-      (fun x -> backtranslate (extend t1 g) body t2 hbody (stack fs_g x)) in
+      (fun x -> backtranslate hbody (stack fs_g x)) in
     w
-  | EApp e1 e2 ->
-    let TyApp #_ #_ #_ #t1 #t2 h1 h2 = h in
+  | EApp _ _ ->
+    let TyApp #t1 #t2 h1 h2 = h in
     assert ((get_Type t) == (get_Type t2));
-    let v1 : get_Type (t1 ^-> t2) = backtranslate g e1 (t1 ^-> t2) h1 fs_g in
-    let v2 : get_Type t1 = backtranslate g e2 t1 h2 fs_g in
+    let v1 : get_Type (t1 ^-> t2) = backtranslate h1 fs_g in
+    let v2 : get_Type t1 = backtranslate h2 fs_g in
     v1 v2
-  | EPair e1 e2 ->
-    let TyPair #_ #_ #_ #t1 #t2 h1 h2 = h in
-    let v1 = backtranslate g e1 t1 h1 fs_g in
-    let v2 = backtranslate g e2 t2 h2 fs_g in
+  | EPair _ _ ->
+    let TyPair h1 h2 = h in
+    let v1 = backtranslate h1 fs_g in
+    let v2 = backtranslate h2 fs_g in
     (v1, v2)
-  | EFst e ->
-    let TyFst #_ #_ #t1 #t2 h1 = h in
-    let v = backtranslate g e (t1 ^* t2) h1 fs_g in
-    fst #(get_Type t1) #(get_Type t2) v
-  | ESnd e ->
-    let TySnd #_ #_ #t1 #t2 h1 = h in
-    let v = backtranslate g e (t1 ^* t2) h1 fs_g in
-    snd #(get_Type t1) #(get_Type t2) v
+  | EFst _ ->
+    let TyFst #t1 h1 = h in
+    fst #(get_Type t1) (backtranslate h1 fs_g)
+  | ESnd _ ->
+    let TySnd #t2 h1 = h in
+    snd #_ #(get_Type t2) (backtranslate h1 fs_g)
+  | EInl _ ->
+    let TyInl t2 h = h in
+    Inl #_ #(get_Type t2) (backtranslate h fs_g)
+  | EInr _ ->
+    let TyInr t1 h = h in
+    Inr #(get_Type t1) (backtranslate h fs_g)
+  | ECase _ _ _ ->
+    let TyCase hcond hinlc hinrc = h in
+    match backtranslate hcond fs_g with
+    | Inl x -> backtranslate hinlc (stack fs_g x)
+    | Inr x -> backtranslate hinrc (stack fs_g x)
 
 #push-options "--split_queries always"
-let rec lem_backtranslate g e t (h:typing g e t) =
+let rec lem_backtranslate #g #e #t (h:typing g e t) =
    match e with
   | EUnit -> equiv_unit g
   | EVar x -> equiv_var g x
   | EApp e1 e2 ->
-    let TyApp #_ #_ #_ #t1 #t2 h1 h2 = h in
+    let TyApp h1 h2 = h in
     lem_app_fv_in_env g e1 e2;
-    lem_backtranslate g e1 (t1 ^-> t2) h1;
-    lem_backtranslate g e2 t1 h2;
-    let fs_e1 = (backtranslate g e1 (t1 ^-> t2) h1) in
-    let fs_e2 = (backtranslate g e2 t1 h2) in
+    lem_backtranslate h1;
+    lem_backtranslate h2;
+    let fs_e1 = backtranslate h1 in
+    let fs_e2 = backtranslate h2 in
     equiv_app fs_e1 fs_e2 e1 e2
-  | ELam body ->
-    let TyLam #_ #body #t1 #t2 hbody = h in
+  | ELam _ -> (** TODO/Abigail: check if one can refactor this with equiv_lam **)
+    let TyLam #t1 #t2 #body hbody = h in
     lem_lam_fv_in_env g body t1;
-    lem_backtranslate (extend t1 g) body t2 hbody;
-    assert (equiv t2 (backtranslate (extend t1 g) body t2 hbody) body);
-    assert (forall b (s:gsub (extend t1 g) b) (fsG:eval_env (extend t1 g)). fsG ∽ s ==> t2 ⦂ ((backtranslate (extend t1 g) body t2 hbody) fsG, gsubst s body));
+    lem_backtranslate hbody;
+    assert (equiv t2 (backtranslate hbody) body);
+    assert (forall b (s:gsub (extend t1 g) b) (fsG:eval_env (extend t1 g)). fsG ∽ s ==> t2 ⦂ ((backtranslate hbody) fsG, gsubst s body));
     let g' = extend t1 g in
-    introduce forall b (s:gsub g b) (fsG:eval_env g). fsG ∽ s ==> (t1 ^-> t2) ⦂ ((fun x -> backtranslate (extend t1 g) body t2 hbody (stack fsG x)), gsubst s (ELam body)) with
+    introduce forall b (s:gsub g b) (fsG:eval_env g). fsG ∽ s ==> (t1 ^-> t2) ⦂ ((fun x -> backtranslate hbody (stack fsG x)), gsubst s (ELam body)) with
       begin
-      let f : (get_Type t1) -> (get_Type t2) = (fun x -> backtranslate (extend t1 g) body t2 hbody (stack fsG x)) in
+      let f : (get_Type t1) -> (get_Type t2) = (fun x -> backtranslate hbody (stack fsG x)) in
       let body' = subst (sub_elam s) body in
       assert (gsubst s (ELam body) == ELam body');
       introduce  fsG ∽ s ==> (t1 ^-> t2) ⦂ (f, ELam body') with _.
@@ -156,33 +188,57 @@ let rec lem_backtranslate g e t (h:typing g e t) =
   | ETrue -> equiv_true g
   | EFalse -> equiv_false g
   | EIf e1 e2 e3 ->
-    let TyIf #_ #_ #_ #_ #t h1 h2 h3 = h in
+    let TyIf h1 h2 h3 = h in
     lem_if_fv_in_env g e1 e2 e3;
-    lem_backtranslate g e1 qBool h1;
-    lem_backtranslate g e2 t h2;
-    lem_backtranslate g e3 t h3;
-    let fs_e1 = (backtranslate g e1 qBool h1) in
-    let fs_e2 = (backtranslate g e2 t h2) in
-    let fs_e3 = (backtranslate g e3 t h3) in
+    lem_backtranslate h1;
+    lem_backtranslate h2;
+    lem_backtranslate h3;
+    let fs_e1 = (backtranslate h1) in
+    let fs_e2 = (backtranslate h2) in
+    let fs_e3 = (backtranslate h3) in
     equiv_if fs_e1 fs_e2 fs_e3 e1 e2 e3
   | EPair e1 e2 ->
-    let TyPair #_ #_ #_ #t1 #t2 h1 h2 = h in
+    let TyPair h1 h2 = h in
     lem_pair_fv_in_env g e1 e2;
-    lem_backtranslate g e1 t1 h1;
-    lem_backtranslate g e2 t2 h2;
-    let fs_e1 = (backtranslate g e1 t1 h1) in
-    let fs_e2 = (backtranslate g e2 t2 h2) in
+    lem_backtranslate h1;
+    lem_backtranslate h2;
+    let fs_e1 = (backtranslate h1) in
+    let fs_e2 = (backtranslate h2) in
     equiv_pair fs_e1 fs_e2 e1 e2
   | EFst e12 ->
-    let TyFst #_ #_ #t1 #t2 h1 = h in
+    let TyFst h1 = h in
     lem_fst_fv_in_env g e12;
-    lem_backtranslate g e12 (t1 ^* t2) h1;
-    let fs_e12 = (backtranslate g e12 (t1 ^* t2) h1) in
+    lem_backtranslate h1;
+    let fs_e12 = (backtranslate h1) in
     equiv_pair_fst_app fs_e12 e12
   | ESnd e12 ->
-    let TySnd #_ #_ #t1 #t2 h1 = h in
+    let TySnd h1 = h in
     lem_snd_fv_in_env g e12;
-    lem_backtranslate g e12 (t1 ^* t2) h1;
-    let fs_e12 = (backtranslate g e12 (t1 ^* t2) h1) in
+    lem_backtranslate h1;
+    let fs_e12 = (backtranslate h1) in
     equiv_pair_snd_app fs_e12 e12
+  | EInl e' ->
+    let TyInl t2 h' = h in
+    assume (fv_in_env g e');
+    lem_backtranslate h';
+    let fs_e' = backtranslate h' in
+    admit ()
+  | EInr e' ->
+    let TyInr t1 h' = h in
+    assume (fv_in_env g e');
+    lem_backtranslate h';
+    let fs_e' = backtranslate h' in
+    admit ()
+  | ECase cond inlc inrc ->
+    let TyCase #t1 #t2 hcond hinlc hinrc = h in
+    assume (fv_in_env g cond);
+    assume (fv_in_env (extend t1 g) inlc);
+    assume (fv_in_env (extend t2 g) inrc);
+    lem_backtranslate hcond;
+    lem_backtranslate hinlc;
+    lem_backtranslate hinrc;
+    let fs_cond = backtranslate hcond in
+    let fs_inlc = backtranslate hinlc in
+    let fs_inrc = backtranslate hinrc in
+    admit ()
 #pop-options
